Add: soundness of the tableaux

theories/Proofs.v
@@ -39,10 +39,12 @@ Section Tableaux.
   (** A [Branch] of a tableau is a succession of [BranchingStep]s. *)
   Definition Branch := list BranchingStep.
 
+  Definition EmptyBranch : Branch := [].
+
   (** A [Branch] [is_branch_of] a [TableauTree] whenever the list of branching steps describes
       a path from the root of the [TableauTree] to a node without children. *)
   Inductive is_branch_of : Branch -> TableauTree -> Prop :=
-  | is_branch_of_nil : forall (Gamma : list Form), is_branch_of [] (Node Leaf Gamma Leaf)
+  | is_branch_of_nil : forall (Gamma : list Form), is_branch_of EmptyBranch (Node Leaf Gamma Leaf)
   | is_branch_of_left :
     forall (T1 T2 : TableauTree) (Gamma : list Form) (B : Branch),
       is_branch_of B T1 -> is_branch_of (Left :: B) (Node T1 Gamma T2)
@@ -70,34 +72,41 @@ Section Tableaux.
 
   Fixpoint expand_tableau_branch__aux (left_forms right_forms : option (list Form))
     (B : Branch) (T : TableauTree) : option TableauTree :=
-    match B with
-    | [] =>
-        match T with
-        | Node Leaf Gamma Leaf => Some (Node (mkOptionalNode left_forms) Gamma (mkOptionalNode right_forms))
-        | _ => None
-        end
-    | b :: B =>
-        match T with
-        | Leaf => None
-        | Node T1 Gamma T2 =>
-            match b with
-            | Left => expand_tableau_branch__aux left_forms right_forms B T1 >>=
-                       (fun T1 => Some (Node T1 Gamma T2))
-            | Right => expand_tableau_branch__aux left_forms right_forms B T2 >>=
-                        (fun T2 => Some (Node T1 Gamma T2))
-            end
-        end
+    match B, T with
+    | [], Node Leaf Gamma Leaf =>
+        Some (Node (mkOptionalNode left_forms) Gamma (mkOptionalNode right_forms))
+    | Left :: B, Node T1 Gamma T2 =>
+        expand_tableau_branch__aux left_forms right_forms B T1 >>=
+          (fun T1 => Some (Node T1 Gamma T2))
+    | Right :: B, Node T1 Gamma T2 =>
+        expand_tableau_branch__aux left_forms right_forms B T2 >>=
+          (fun T2 => Some (Node T1 Gamma T2))
+    | _, _ => None
     end.
+
+  Lemma expand_tableau_branch_left :
+    forall (Gamma : list Form) (T1 T1' T2 : TableauTree) (B : Branch)
+      (left_forms right_forms : option (list Form)),
+      expand_tableau_branch__aux left_forms right_forms B T1 = Some T1' ->
+      expand_tableau_branch__aux left_forms right_forms (Left :: B) (Node T1 Gamma T2) =
+        Some (Node T1' Gamma T2).
+  Proof using Type. intros ??????? e; cbn; rewrite e //. Qed.
+
+  Lemma expand_tableau_branch_right :
+    forall (Gamma : list Form) (T1 T2 T2' : TableauTree) (B : Branch)
+      (left_forms right_forms : option (list Form)),
+      expand_tableau_branch__aux left_forms right_forms B T2 = Some T2' ->
+      expand_tableau_branch__aux left_forms right_forms (Right :: B) (Node T1 Gamma T2) =
+        Some (Node T1 Gamma T2').
+  Proof using Type. intros ??????? e; cbn; rewrite e //. Qed.
 
   (** The [context] of a branch is the list of all the formulas of a branch. *)
   Fixpoint get_context (B : Branch) (T : TableauTree) : list Form :=
-    match T with
-    | Leaf => []
-    | Node T1 Gamma T2 => Gamma ++ (match B with
-                           | [] => []
-                           | Left :: B => get_context B T1
-                           | Right :: B => get_context B T2
-                           end)%list
+    match B, T with
+    | [], Node Leaf Gamma Leaf => Gamma
+    | Left :: B, Node T1 Gamma _ => (Gamma ++ get_context B T1)%list
+    | Right :: B, Node _ Gamma T2 => (Gamma ++ get_context B T2)%list
+    | _, _ => []
     end.
 
   (** Actually, a [Tableau_] also keeps in memory the Skolem symbols introduced. *)
@@ -183,6 +192,39 @@ Section Tableaux.
       + inversion e.
   Qed.
 
+  Lemma is_branch_of_extend_oth :
+    forall (T T' : TableauTree) (B B' : Branch) (l l' : option (list Form)),
+      is_branch_of B' T -> is_branch_of B T -> B <> B' ->
+      expand_tableau_branch__aux l l' B T = Some T' -> is_branch_of B' T'.
+  Proof using Type.
+    intros ????. revert T T' B'. induction B as [|b B IHB];
+      intros ????? hbranchof' hbranchof n e;  destruct B' as [|b' B'].
+    - easy.
+    - inversion hbranchof; subst; inversion hbranchof'; inversion H0.
+    - inversion hbranchof'; subst; inversion hbranchof; inversion H0.
+    - destruct b.
+      + inversion hbranchof. destruct (expand_tableau_branch__aux l l' B T1) eqn:e1.
+        * erewrite <-H1, expand_tableau_branch_left in e; eauto. destruct b'.
+          -- injection e => <-. apply is_branch_of_left. eapply IHB; eauto.
+             ++ inversion hbranchof'; subst; auto.
+                injection H4 => _ _ <- //.
+             ++ congruence.
+          -- rewrite -H1 in hbranchof'. inversion hbranchof'; subst.
+             injection e => <-. now apply is_branch_of_right.
+        * cbn in e. destruct T; try easy. injection H1 => _ _ eT1. rewrite eT1 in e1.
+          rewrite e1 in e. inversion e.
+      + inversion hbranchof. destruct (expand_tableau_branch__aux l l' B T2) eqn:e2.
+        * erewrite <- H1, expand_tableau_branch_right in e; eauto. destruct b'.
+          -- rewrite -H1 in hbranchof'. inversion hbranchof'; subst.
+             injection e => <-. now apply is_branch_of_left.
+          -- injection e => <-. apply is_branch_of_right. eapply IHB; eauto.
+             ++ inversion hbranchof'; subst; auto.
+                injection H4 => <- _ _ //.
+             ++ congruence.
+        * cbn in e. destruct T; try easy. injection H1 => eT2 _ _. rewrite eT2 in e2.
+          rewrite e2 in e. inversion e.
+  Qed.
+
   Lemma get_context_extend_left :
     forall (T T' : TableauTree) (B : Branch) (Gamma l : list Form) (l' : option (list Form)),
       is_branch_of B T -> expand_tableau_branch__aux (Some l) l' B T = Some T' ->
@@ -190,9 +232,9 @@ Section Tableaux.
   Proof using Type.
     intro T. induction T; intros ????? hbranchof e eT; destruct B.
     - inversion e.
-    - inversion e.
+    - inversion e; destruct b; easy.
     - inversion hbranchof; subst. cbn in e.
-      injection e => <-; cbn. now rewrite !app_nil_r.
+      injection e => <- //.
     - destruct b; cbn.
       + inversion hbranchof; subst.
         cbn in e. destruct (expand_tableau_branch__aux (Some l) l' B T1) eqn:eT1.
@@ -213,9 +255,9 @@ Section Tableaux.
   Proof using Type.
     intro T. induction T; intros ????? hbranchof e eT; destruct B.
     - inversion e.
-    - inversion e.
+    - inversion e. destruct b; easy.
     - inversion hbranchof; subst. cbn in e.
-      injection e => <-; cbn. now rewrite !app_nil_r.
+      injection e => <-; now cbn.
     - destruct b; cbn.
       + inversion hbranchof; subst.
         cbn in e. destruct (expand_tableau_branch__aux l (Some l') B T1) eqn:eT1.
@@ -229,6 +271,41 @@ Section Tableaux.
         * inversion e.
   Qed.
 
+  Lemma get_context_extend_oth :
+    forall (T T' : TableauTree) (B B' : Branch) (l l' : option (list Form)),
+      is_branch_of B T -> is_branch_of B' T -> B <> B' ->
+      expand_tableau_branch__aux l l' B T = Some T' -> get_context B' T = get_context B' T'.
+  Proof using Type.
+    intros ?? B. revert T T'. induction B as [|b B IHB]; intros ????? hbranchof hbranchof' n e;
+      destruct B' as [|b' B'].
+    - easy.
+    - inversion hbranchof; subst. inversion hbranchof'; subst; inversion H0.
+    - inversion hbranchof'; subst. inversion hbranchof; subst; inversion H0.
+    - destruct b, b'; cbn.
+      + inversion hbranchof; subst.
+        destruct (expand_tableau_branch__aux l l' B T1) eqn:e1.
+        * erewrite expand_tableau_branch_left in e; eauto.
+          injection e => <-. erewrite IHB; eauto.
+          -- now inversion hbranchof'.
+          -- congruence.
+        * cbn in e; rewrite e1 in e; inversion e.
+      + inversion hbranchof'; subst.
+        destruct (expand_tableau_branch__aux l l' B T1) eqn:e1.
+        * erewrite expand_tableau_branch_left in e; eauto. injection e => <- //.
+        * cbn in e; rewrite e1 in e; inversion e.
+      + inversion hbranchof'; subst.
+        destruct (expand_tableau_branch__aux l l' B T2) eqn:e2.
+        * erewrite expand_tableau_branch_right in e; eauto. injection e => <- //.
+        * cbn in e; rewrite e2 in e; inversion e.
+      + inversion hbranchof; subst.
+        destruct (expand_tableau_branch__aux l l' B T2) eqn:e2.
+        * erewrite expand_tableau_branch_right in e; eauto.
+          injection e => <-. erewrite IHB; eauto.
+          -- now inversion hbranchof'.
+          -- congruence.
+        * cbn in e; rewrite e2 in e; inversion e.
+  Qed.
+
   (** An optional list of formulas is satisfied either if it is none or if the list is
       satisfied. *)
   Definition is_optional_satisfied
@@ -240,63 +317,105 @@ Section Tableaux.
 
   (** If a satisfiable tableau is extended with lists of formulas of which one of them is also
       satisfied by the same model, then the extended tableau is also satisfiable. *)
+  Lemma is_satisfiable_extend_gen :
+    forall (M M' : Model pred func) (T T' : Tableau_) (B : Branch) (l l' : option (list Form))
+      (mu' : env M' var) (f : env M' var -> env M var),
+      is_branch_of B T -> expand_tableau_branch__aux l l' B T = Some (tree T') ->
+      (forall (F : Form), [[ M # [] # f mu' '|= F ]] ->
+                     [[ M' # [] # mu' '|= F ]]) ->
+      ([[ M # [] # (f mu') '|= ls_to_form (get_context B T) ]] ->
+       is_optional_satisfied M' mu' l \/ is_optional_satisfied M' mu' l') ->
+      (exists_satisfied_branch M (f mu') T) ->
+      exists_satisfied_branch M' mu' T'.
+  Proof using Type.
+    intros ?? [T symbs] [T' symbs'] ????? hbranchof e hcsv hsatlr (B & hbranchB & hsatB);
+      cbn in e.
+
+    destruct (B == B0); subst.
+
+    (* Case: the branch that was satisfied is, in fact, [B0]. *)
+    - destruct (hsatlr hsatB) as [hsatl | hsatr].
+
+      (* Case: the extension with the formulas on the left is satisfied. *)
+      + destruct l.
+        * exists (B0 ++ [Left])%list; split; cbn.
+          -- destruct (expand_tableau_branch__aux (Some l) l' B0 T) eqn:eT.
+             ++ eapply is_branch_of_extend_left; eauto.
+                injection e => <-; eauto.
+             ++ inversion e.
+          -- destruct (expand_tableau_branch__aux (Some l) l' B0 T) eqn:eT.
+             ++ injection e => eT'. rewrite eT' in eT. erewrite get_context_extend_left; eauto.
+                cbn. unfold interpret; rewrite (ls_to_form_app (get_context B0 T) l M' [] mu').
+                cbn. intros [hnB0 | hl]; auto. now apply hnB0, hcsv.
+             ++ inversion e.
+        * now cbn in hsatl.
+
+      (* Case: the extension with the formulas on the right is satisfied. *)
+      + destruct l'.
+        * exists (B0 ++ [Right])%list; split; cbn.
+          -- destruct (expand_tableau_branch__aux l (Some l0) B0 T) eqn:eT.
+             ++ eapply is_branch_of_extend_right; eauto.
+                injection e => <-; eauto.
+             ++ inversion e.
+          -- destruct (expand_tableau_branch__aux l (Some l0) B0 T) eqn:eT.
+             ++ injection e => eT'; rewrite eT' in eT.
+                erewrite get_context_extend_right; eauto.
+                cbn; unfold interpret. rewrite (ls_to_form_app (get_context B0 T) l0 M' [] mu').
+                cbn. intros [hnB0 | hl0]; auto. now apply hnB0, hcsv.
+             ++ inversion e.
+
+        * inversion hsatr.
+
+      (* Case: the branch that was satisfied is not [B0]. *)
+    - destruct (expand_tableau_branch__aux l l' B0 T) eqn:eT'.
+      + injection e => <-. exists B; split.
+        * apply is_branch_of_extend_oth with (T := T) (B := B0) (l := l) (l' := l'); auto.
+        * cbn in *. rewrite -(get_context_extend_oth T t B0 B l l' hbranchof hbranchB); try easy.
+          now apply hcsv.
+      + inversion e.
+  Qed.
+
   Lemma is_satisfiable_extend :
     forall (M : Model pred func) (mu : env M var) (T T' : Tableau_) (B : Branch)
       (l l' : option (list Form)),
       is_branch_of B T -> expand_tableau_branch l l' B T = Some T' ->
-      is_optional_satisfied M mu l \/ is_optional_satisfied M mu l' ->
+      ([[ M # [] # mu '|= ls_to_form (get_context B T) ]] ->
+       is_optional_satisfied M mu l \/ is_optional_satisfied M mu l') ->
       exists_satisfied_branch M mu T -> exists_satisfied_branch M mu T'.
-  Proof.
-    intros ?? [T symbs] [T' symbs'] ??? hbranchof e [hsatl | hsatl'] (B & hbranchB & hsatB);
-      cbn in e.
+  Proof using Type.
+    intros ??????? hbranchof e himp hb.
+    eapply is_satisfiable_extend_gen with (f := fun x => x); eauto.
+    cbn in *; destruct (expand_tableau_branch__aux l l' B T); try easy.
+    injection e => <- //.
+  Qed.
 
-    (* Case: the extension with the formulas on the left is satisfied. *)
-    - destruct (B == B0).
+  Lemma is_on_branch_in_context :
+    forall (T : Tableau_) (B : Branch) (F : Form),
+      is_branch_of B T -> is_on_branch F B T -> F \in get_context B T.
+  Proof using Type.
+    intros ??? hbranchof honbranch. induction honbranch.
+    - destruct B; cbn in *.
+      + inversion hbranchof; now subst.
+      + destruct b; apply in_or_app; now left.
+    - cbn. apply in_or_app; right. apply IHhonbranch. now inversion hbranchof.
+    - cbn. apply in_or_app; right. apply IHhonbranch. now inversion hbranchof.
+  Qed.
 
-      (* Case: the branch that was satisfied is, in fact, [B0]. *)
-      + destruct l.
-        * exists (List.app B [Left]); split; cbn.
-          -- rewrite e0. destruct (expand_tableau_branch__aux (Some l) l' B0 T) eqn:eT.
-             ++ eapply is_branch_of_extend_left; eauto.
-                injection e => ? <-; eauto.
-             ++ inversion e.
-          -- rewrite -e0 in e. destruct (expand_tableau_branch__aux (Some l) l' B T) eqn:eT.
-             ++ injection e => _ eT'. rewrite eT' in eT. erewrite get_context_extend_left; eauto.
-                cbn. unfold interpret; rewrite (ls_to_form_app (get_context B T) l M [] mu).
-                cbn. intros [hnB | hl]; auto.
-             ++ inversion e.
-        * now cbn in hsatl.
-
-      (* Case: the branch that was satisfied is not [B0]. *)
-      + exists B; split; admit.
-
-    (* Case: the extension with the formulas on the right is satisfied. *)
-    - destruct (B == B0).
-
-      (* Case: the branch that was satisfied is, in fact, [B0]. *)
-      + destruct l'.
-        * exists (B ++ [Right])%list; split; cbn.
-          -- rewrite e0. destruct (expand_tableau_branch__aux l (Some l0) B0 T) eqn:eT.
-             ++ eapply is_branch_of_extend_right; eauto.
-                injection e => ? <-; eauto.
-             ++ inversion e.
-          -- rewrite -e0 in e. destruct (expand_tableau_branch__aux l (Some l0) B T) eqn:eT.
-             ++ injection e => _ eT'; rewrite eT' in eT.
-                erewrite get_context_extend_right; eauto.
-                cbn; unfold interpret. rewrite (ls_to_form_app (get_context B T) l0 M [] mu).
-                cbn. intros [hnB | hl0]; auto.
-             ++ inversion e.
-
-        * inversion hsatl'.
-
-      (* Case: the branch that was satisfied is not [B0]. *)
-      + exists B; split; admit.
-  Admitted.
+  Lemma is_on_satisfiable_branch :
+    forall {T : Tableau_} {B : Branch} {F : Form} {M : Model pred func} {mu : env M var},
+      is_branch_of B T -> is_on_branch F B T -> [[ M # [] # mu '|= ls_to_form (get_context B T) ]] ->
+      [[ M # [] # mu '|= F ]].
+  Proof using Type.
+    intros ????? hbranchof honbranch hsat.
+    have h := in_form_list_interp _ hsat.
+    apply h, is_on_branch_in_context; auto.
+  Qed.
 End Tableaux.
 
 Arguments tree {_ _ _ _}.
 Arguments symbols {_ _ _ _}.
 Arguments is_tableau_closed {_ _ _ _ _} _ _.
+Arguments is_tableau_satisfiable {_ _ _ _} _.
 Arguments exists_satisfied_branch {_ _ _ _} _ _ _.
 
 (** ** Expansion rules *)
@@ -336,7 +455,7 @@ Section ExpansionRules.
     forall (T T' : Tableau) (B : Branch) (F : Form) (t : Term)
       (hsko : sko t (Neg (All F)) (symbols T) (get_context B T) = true),
       is_branch_of B T -> is_on_branch (Neg (All F)) B T ->
-      expand_tableau_branch__aux (Some [F{0 \to t}]) None B T = Some (tree T') ->
+      expand_tableau_branch__aux (Some [Neg F{0 \to t}]) None B T = Some (tree T') ->
       symbols T' = add_symbol (symbol sko hsko) (Neg (All F)) (symbols T) ->
       T |> T'
   where "T |> T'" := (ExpansionStep T T').
@@ -361,6 +480,7 @@ Section ExpansionRules.
 End ExpansionRules.
 
 Arguments ExpansionStep {_ _ _ _} _ _.
+Arguments is_expansion_sequence {_ _ _ _} _.
 Notation "T |> T'" := (ExpansionStep T T').
 
 (** ** Soundness *)
@@ -392,15 +512,15 @@ Section Soundness.
   Qed.
 
   (** Then, we show that every expansion sequence starting from a satisfiable tableau is
-      satisfiable. We even show that there exists one model that satisfies every element
-      of the sequence. *)
+      satisfiable. We could even show the stronger property that there exists a model satisfying
+      all the consecutive tableaux of the expansion. *)
 
   (** We start by showing that applying an [ExpansionStep] on a satisfiable tableau keeps
       satisfiability. *)
-  Lemma subject_reduction :
+  Lemma satisfiable_expansion_satisfiable :
     forall (T T' : Tableau),
-      is_tableau_satisfiable sko T -> (T |> T') ->
-      is_tableau_satisfiable sko T'.
+      is_tableau_satisfiable T -> (T |> T') ->
+      is_tableau_satisfiable T'.
   Proof using set_nat.
     intros T T' hsat hred. destruct hred as
       [ T T' B F hbranchof hcontains e |
@@ -412,1048 +532,106 @@ Section Soundness.
     (* Case: [Neg (Neg F)] *)
     - destruct hsat as (M & hsat). exists M; intro mu. specialize (hsat mu).
       eapply is_satisfiable_extend; eauto. left.
-      intros [hnF | contra]; firstorder.
-      (* easy *)
-
-eapply is_satisfiable_is_satisfiable_add_in_branch; eauto.
-      apply equiv_imply. symmetry; apply neg_neg_equiv.
+      intros [hnF | contra].
+      + now apply (is_on_satisfiable_branch sko hbranchof hcontains H).
+      + cbn in contra; apply contra; now intro.
 
     (* Case: [Neg (Or F1 F2)] *)
-    - eapply is_satisfiable_is_satisfiable_add_in_branch with
-        (F := Neg (Or F1 F2)) (T := add_in_branch T i (Neg F1)).
-      + eapply add_in_branch_get; eauto.
-      + eapply is_satisfiable_is_satisfiable_add_in_branch; eauto.
-        intros M sigma hinterp hF1. apply hinterp. now left.
-      + now apply branch_contains_add.
-      + intros M sigma hinterp hF2. apply hinterp. now right.
+    - destruct hsat as (M & hsat). exists M; intro mu. specialize (hsat mu).
+      eapply is_satisfiable_extend; eauto. left.
+      intros [hF1 | hnnF ].
+      + apply hF1; intro.
+        apply (is_on_satisfiable_branch sko hbranchof hcontains H); now left.
+      + apply hnnF; intros [hF2 | contra].
+        * apply hF2; intro.
+          apply (is_on_satisfiable_branch sko hbranchof hcontains H); now right.
+        * apply contra. now intro.
 
     (* Case: [Or F1 F2] *)
-    - apply is_satisfiable_is_satisfiable_or; auto.
+    - destruct hsat as (M & hsat). exists M; intro mu. specialize (hsat mu).
+      eapply is_satisfiable_extend; eauto.
+      intro hinterp; have [hF1 | hF2] := is_on_satisfiable_branch sko hbranchof hcontains hinterp.
+      + left; cbn. intros [hnF1 | contra]; try easy. apply contra; now intro.
+      + right; cbn. intros [hnF2 | contra]; try easy. apply contra; now intro.
 
     (* Case: [All F] *)
-    - eapply is_satisfiable_is_satisfiable_add_in_branch; eauto.
-      apply instantiate_imply_all. unfold isLocallyClosed; now cbn.
+    - destruct hsat as (M & hsat). exists M; intro mu. specialize (hsat mu).
+      eapply is_satisfiable_extend; eauto. left.
+      intros [hnF | contra].
+      + have hall := is_on_satisfiable_branch sko hbranchof hcontains H.
+        apply hnF, instantiate_imply_all; auto.
+        now cbn.
+      + cbn in contra; apply contra; now intro.
 
     (* Case: [Neg (All F)] *)
     - destruct hsat as (M & hsat0).
-      destruct (is_sko_sound H M) as (interp & hinterpsko & hinterp).
+      destruct (is_sko_sound hsko M) as (interp & hinterpsko & hinterp).
       exists (ReplacementModel M interp); intro mu.
-      specialize (hsat0 mu). destruct hsat0 as (B0 & hin & hinterp0).
-      apply In_nth_error in hin; destruct hin as (k & ek).
-      destruct (i == k); subst.
-      + exists (B ,, Neg F {0 \to t}); split.
-        * unfold add_in_branch. rewrite H0.
-          eapply In_replace_nth; eauto.
-        * have eB0 : B = B0.
-          { unfold nth_branch_of in H0; rewrite H0 in ek; now injection ek. }
-          intros [hnF | hB].
-          -- apply hnF, hinterpsko.
-             eapply in_form_list_interp; eauto.
-             now rewrite eB0.
-          -- rewrite eB0 in hB; now apply hB, hinterp.
-      + exists B0; split.
-        * unfold add_in_branch. rewrite H0.
-          eapply In_replace_nth'; eauto.
-        * now apply hinterp.
+      eapply is_satisfiable_extend_gen with (M := M) (M' := ReplacementModel M interp)
+                                            (f := fun x => x); eauto.
+      intro hinterp'; left; cbn. intros [ hnF | contra ].
+      + apply hnF, hinterpsko.
+        eapply is_on_satisfiable_branch; eauto.
+      + apply contra; now intro.
   Qed.
 
-End Soundness.
-
-(** ** Contexts *)
-
-(** As we want to keep a [sko_record] in the contexts, contexts get parameterized by
-    skolemization instances. *)
-Section Context.
-  Context `{set_nat : set nat} {pred func var : Atom}.
-
-  Let Form := Form_ pred func var.
-
-  Definition Con_ := list (Form_ pred func var).
-
-  Definition empty_ctx : Con_ := [].
-  Definition in_ctx (F : Form) (Gamma : Con_) : Prop := List.In F Gamma.
-  Fixpoint mem_ctx (F : Form) (Gamma : Con_) : bool :=
-    match Gamma with
-    | [] => false
-    | G :: Gamma => eqb F G || mem_ctx F Gamma
-    end.
-
-  Lemma mem_ctx_in_ctx :
-    forall (Gamma : Con_) (F : Form), mem_ctx F Gamma = true <-> in_ctx F Gamma.
-  Proof using Type.
-    intros ??; induction Gamma as [|G Gs IHGs].
-    - now cbn.
-    - cbn; split.
-      + intros h%Bool.orb_true_elim. destruct h.
-        * rewrite eqbIsEq in e. now left.
-        * rewrite IHGs in e. now right.
-      + intros [e | hin].
-        * rewrite e EqBool_refl. now cbn.
-        * apply Bool.orb_true_intro. right. rewrite IHGs //.
-  Qed.
-
-  Definition extend_ctx (Gamma : Con_) (F : Form) : Con_ := F :: Gamma.
-
-  #[global] Instance fv_ctx : @FV var Con_ := ltac:(typeclasses eauto).
-
-  Fixpoint subst_ctx_ (Gamma : Con_) (sigma : Substitution var (Term_ func var)) : Con_ :=
-    match Gamma with
-    | [] => []
-    | F :: Fs => F@[sigma] :: subst_ctx_ Fs sigma
-    end.
-
-  #[global] Instance subst_ctx : Subst Con_ (Term_ func var) :=
-    subst_ctx_.
-
-  Definition ctx_to_form (Gamma : Con_) := ls_to_form Gamma.
-
-  Definition sub_ctx (Gamma Gamma' : Con_) :=
-    forall (F : Form), in_ctx F Gamma -> in_ctx F Gamma'.
-
-  Definition is_sub_ctx (Gamma Gamma' : Con_) : bool :=
-    forallb (fun F => mem_ctx F Gamma') Gamma.
-
-  Lemma is_sub_ctx_sound :
-    forall (Gamma Gamma' : Con_),
-      is_sub_ctx Gamma Gamma' = true -> sub_ctx Gamma Gamma'.
-  Proof using Type.
-    intros ?? e. unfold is_sub_ctx in e. induction Gamma as [|F Gamma IHGamma].
-    - now intros F contra.
-    - cbn in e |- *. apply andb_prop in e. intros G [e' | hin].
-      + subst. rewrite -mem_ctx_in_ctx. apply e.
-      + apply IHGamma.
-        * apply e.
-        * apply hin.
-  Qed.
-
-  Lemma is_sub_ctx_complete :
-    forall (Gamma Gamma' : Con_),
-      sub_ctx Gamma Gamma' -> is_sub_ctx Gamma Gamma' = true.
-  Proof using Type.
-    intros ?? hsub. induction Gamma as [|F Gamma IHGamma]; cbn; auto.
-    apply andb_true_intro; split.
-    - rewrite mem_ctx_in_ctx. apply hsub. now left.
-    - apply IHGamma. intros G hin. apply hsub. now right.
-  Qed.
-
-  Lemma extend_sub_ctx :
-    forall (Gamma Gamma' : Con_) (F : Form),
-      sub_ctx Gamma Gamma' -> sub_ctx (F :: Gamma) (F :: Gamma').
-  Proof using Type.
-    intros ??? hsub; unfold sub_ctx in hsub |- *.
-    intros G [-> | hG].
-    - now left.
-    - right; now apply hsub.
-  Qed.
-
-  Lemma cons_sub_ctx :
-    forall (Gamma Gamma' : Con_) (F : Form),
-      sub_ctx Gamma Gamma' -> sub_ctx Gamma (F :: Gamma').
-  Proof using Type.
-    intros ??? hsub. unfold sub_ctx in hsub |- *; cbn.
-    intros G hin; right. now apply hsub.
-  Qed.
-
-  Lemma sub_ctx_cong :
-    forall (Gamma Gamma' : Con_) (F G : Form),
-      sub_ctx Gamma (F :: Gamma') -> sub_ctx (G :: Gamma) (F :: G :: Gamma').
-  Proof using Type.
-    intros ???? hsub H hin. cbn in hin |- *. destruct hin; auto.
-    apply hsub in H0; cbn in H0; destruct H0 as [e | hin]; auto.
-  Qed.
-
-  Lemma sub_ctx_refl :
-    forall (Gamma : Con_), sub_ctx Gamma Gamma.
-  Proof using Type. do 2 intro. tauto. Qed.
-End Context.
-
-Arguments Con_ : clear implicits.
-
-Notation "Gamma ,, A" := (extend_ctx Gamma A) (at level 20).
-Notation "A \in Gamma" := (in_ctx A Gamma) (at level 30).
-Notation "A \subseteq Gamma" := (sub_ctx A Gamma) (at level 30).
-Notation "{{ }}" := (empty_ctx).
-Notation "{{ F }}" := (empty_ctx ,, F).
-Notation "{{ F1 ;; F2 ;; .. ;; Fk }}" :=
-  (extend_ctx .. (extend_ctx (extend_ctx empty_ctx F1) F2) .. Fk).
-
-(** ** Definition of tableaux *)
-Section TableauxProofs.
-  Context `{set_nat : set nat} {pred func var : Atom} (sko : Skolemization_ pred func var).
-
-  Existing Instance fv_ctx.
-
-  Let set_var := set_atom var.
-  Let set_func := set_atom func.
-  Let Con := Con_ pred func var.
-  Let Term := Term_ func var.
-  Let Form := Form_ pred func var.
-  Let sko_record := sko_record sko.
-
-  (** We unset the automatic generation of elimination schemes to get a dependent elimination
-      for the predicate [hasTableau_]. *)
-  Unset Elimination Schemes.
-  Inductive hasTableau_
-    : Con -> sko_record -> Substitution var Term -> Type :=
-
-  (** Axioms *)
-  | hasTableauBot :
-    forall (Gamma : Con) (symbs : sko_record) (sigma : Substitution var Term),
-      (Bot \in Gamma) -> hasTableau_ Gamma symbs sigma
-  | hasTableauContr :
-    forall (Gamma : Con) (symbs : sko_record) (sigma : Substitution var Term)
-      (P P' : Form),
-      P \in Gamma -> P' \in Gamma -> Neg P@[sigma] = P'@[sigma] -> hasTableau_ Gamma symbs sigma
-
-  (** Alpha rules *)
-  | hasTableauNegNeg :
-    forall (Gamma : Con) (symbs : sko_record) (sigma : Substitution var Term) (F : Form),
-      Neg (Neg F) \in Gamma -> hasTableau_ (Gamma ,, F) symbs sigma -> hasTableau_ Gamma symbs sigma
-  | hasTableauNegOr :
-    forall (Gamma : Con) (symbs : sko_record) (sigma : Substitution var Term) (F1 F2 : Form),
-      Neg (Or F1 F2) \in Gamma -> hasTableau_ (Gamma ,, Neg F1 ,, Neg F2) symbs sigma -> hasTableau_ Gamma symbs sigma
-
-  (** Beta rule *)
-  | hasTableauOr :
-    forall (Gamma : Con) (symbs : sko_record) (sigma : Substitution var Term) (F1 F2 : Form),
-      (Or F1 F2) \in Gamma -> hasTableau_ (Gamma ,, F1) symbs sigma -> hasTableau_ (Gamma ,, F2) symbs sigma ->
-      hasTableau_ Gamma symbs sigma
-
-  (** Gamma rule *)
-  | hasTableauAll :
-    forall (Gamma : Con) (symbs : sko_record) (sigma : Substitution var Term) (x : var) (F : Form),
-      (All F) \in Gamma -> hasTableau_ (Gamma ,, F{0 \to Free x}) symbs sigma ->
-      hasTableau_ Gamma symbs sigma
-
-   (** Delta rule *)
-  | hasTableauNegAll :
-    forall (Gamma : Con) (symbs : sko_record) (sigma : Substitution var Term)
-      (F : Form) (t : Term) (Hsko : sko t (Neg (All F)) symbs Gamma = true),
-      (Neg (All F)) \in Gamma ->
-      hasTableau_ (Gamma ,, Neg F{0 \to t}) (add_symbol (symbol sko Hsko) (Neg (All F)) symbs) sigma ->
-      hasTableau_ Gamma symbs sigma.
-  Scheme hasTableau__ind := Induction for hasTableau_ Sort Prop.
-  Scheme hasTableau__rect := Induction for hasTableau_ Sort Type.
-  Set Elimination Schemes.
-
-  Definition hasTableau (Gamma : Con) (sigma : Substitution var Term) : Type :=
-    hasTableau_ Gamma empty_record sigma.
-
-  (** *** Satisfiability of a tableau *)
-
-  (** A tableau is said satisfiable if there exists a branch such that all the formulas of
-      a branch are satisfiable. We can define it as an inductive predicate. *)
-  Inductive is_tableau_satisfiable (M : Model pred func) (mu : env M var)
-    {Gamma : Con} {symbs : sko_record} {sigma : Substitution var Term} :
-    hasTableau_ Gamma symbs sigma -> Prop :=
-
-  | satisfiable_hasTableauContr :
-    forall (P P' : Form) (hin : P \in Gamma) (hin' : P' \in Gamma) (e : Neg P@[sigma] = P'@[sigma]),
-      [[ M # [] # mu '|= ctx_to_form Gamma ]] ->
-      is_tableau_satisfiable M mu (hasTableauContr Gamma symbs sigma P P' hin hin' e)
-
-  | satisfiable_hasTableauNegNeg :
-    forall (F : Form) (hin : Neg (Neg F) \in Gamma) (htab : hasTableau_ (Gamma ,, F) symbs sigma),
-      is_tableau_satisfiable M mu htab ->
-      is_tableau_satisfiable M mu (hasTableauNegNeg Gamma symbs sigma F hin htab)
-
-  | satisfiable_hasTableauNegOr :
-    forall (F1 F2 : Form) (hin : Neg (Or F1 F2) \in Gamma) (htab : hasTableau_ (Gamma ,, Neg F1 ,, Neg F2) symbs sigma),
-      is_tableau_satisfiable M mu htab ->
-      is_tableau_satisfiable M mu (hasTableauNegOr Gamma symbs sigma F1 F2 hin htab)
-
-  | satisfiable_hasTableauOr1 :
-    forall (F1 F2 : Form) (hin : (Or F1 F2) \in Gamma) (htab1 : hasTableau_ (Gamma ,, F1) symbs sigma)
-      (htab2 : hasTableau_ (Gamma ,, F2) symbs sigma),
-      is_tableau_satisfiable M mu htab1 ->
-      is_tableau_satisfiable M mu (hasTableauOr Gamma symbs sigma F1 F2 hin htab1 htab2)
-
-  | satisfiable_hasTableauOr2 :
-    forall (F1 F2 : Form) (hin : (Or F1 F2) \in Gamma) (htab1 : hasTableau_ (Gamma ,, F1) symbs sigma)
-      (htab2 : hasTableau_ (Gamma ,, F2) symbs sigma),
-      is_tableau_satisfiable M mu htab2 ->
-      is_tableau_satisfiable M mu (hasTableauOr Gamma symbs sigma F1 F2 hin htab1 htab2)
-
-  | satisfiable_hasTableauAll :
-    forall (x : var) (F : Form) (hin : (All F) \in Gamma) (htab : hasTableau_ (Gamma ,, F{0 \to Free x}) symbs sigma),
-      is_tableau_satisfiable M mu htab ->
-      is_tableau_satisfiable M mu (hasTableauAll Gamma symbs sigma x F hin htab)
-
-  | satisfiable_hasTableauNegAll :
-    forall (F : Form) (t : Term) (Hsko : sko t (Neg (All F)) symbs Gamma = true)
-      (hin : (Neg (All F)) \in Gamma)
-      (htab : hasTableau_ (Gamma ,, Neg F{0 \to t}) (add_symbol (symbol sko Hsko) (Neg (All F)) symbs) sigma),
-      is_tableau_satisfiable M mu htab ->
-      is_tableau_satisfiable M mu (hasTableauNegAll Gamma symbs sigma F t Hsko hin htab).
-End TableauxProofs.
-Arguments is_tableau_satisfiable {_ _ _ _ _} _ _ {_ _ _} _.
-
-(** ** Some usual properties of tableaux *)
-Section TableauxProperties.
-  Context `{set_nat : set nat} {pred func var : Atom} (sko : Skolemization_ pred func var).
-
-  Let Con := Con_ pred func var.
-  Let Form := Form_ pred func var.
-  Let Term := Term_ func var.
-
-  (** If [Gamma \subseteq Gamma'], then as long as [fv Gamma = fv Gamma'], weakening holds for tableau proofs. *)
-  Lemma weakening :
-    forall (Gamma Gamma' : Con) (symbs : sko_record sko) (sigma : Substitution var Term),
-      fv Gamma = fv Gamma' -> Gamma \subseteq Gamma' ->
-      hasTableau_ sko Gamma symbs sigma ->
-      hasTableau_ sko Gamma' symbs sigma.
-  Proof using Type.
-    intros ????? hsubset htab. generalize dependent Gamma'. induction htab;
-      intros Gamma' efv hsubset.
-    - apply hsubset in i. now apply hasTableauBot.
-    - apply hsubset in i, i0. eapply hasTableauContr.
-      + apply i.
-      + apply i0.
-      + apply e.
-    - apply hsubset in i. eapply hasTableauNegNeg; eauto.
-      apply IHhtab; auto.
-      + cbn. now rewrite efv.
-      + now apply extend_sub_ctx.
-    - apply hsubset in i. eapply hasTableauNegOr; eauto.
-      apply IHhtab; auto.
-      + cbn. rewrite -!union_assoc efv //.
-      + now do 2 apply extend_sub_ctx.
-    - apply hsubset in i. eapply hasTableauOr; eauto.
-      + apply IHhtab1.
-        * cbn. now rewrite efv.
-        * now apply extend_sub_ctx.
-      + apply IHhtab2.
-        * cbn. now rewrite efv.
-        * now apply extend_sub_ctx.
-    - apply hsubset in i. eapply hasTableauAll; eauto.
-      apply IHhtab.
-      2: now apply extend_sub_ctx.
-      cbn. now rewrite efv.
-    - apply hsubset in i.
-      have Hsko' := Hsko. rewrite (sko_con_fv _ Gamma') in Hsko'; auto.
-      apply hasTableauNegAll with (t := t) (Hsko := Hsko'); eauto.
-      have esym : symbol sko Hsko = symbol sko Hsko'.
-      { have e0 : get_symbol t = Some (symbol sko Hsko) by apply symbol_sound.
-        have e1 : get_symbol t = Some (symbol sko Hsko') by apply symbol_sound.
-        destruct t; try inversion e0.
-        cbn in e0, e1; injection e0 => e0'; injection e1 => e1'. now destruct e0', e1'. }
-      rewrite -esym. apply IHhtab.
-      + cbn. now rewrite efv.
-      + now apply extend_sub_ctx.
-  Qed.
-End TableauxProperties.
-
-(** ** Tableaux using expansion *)
-
-(** In this section, we develop the expansion of tableaux. Instead of defining them as inductive
-    trees, we define trees with sequence of expansions corresponding to the rules defined in
-    [hasTableau_]. Then, we can show that having a closed sequence of tableaux expansion is
-    the same as having an [hasTableau_]. Moreover, the satisfiability of a sequence of tableaux
-    is equivalent to the satisfiability of an [hasTableau_], which allow to show e.g. soundness
-    of the [hasTableau_] inductive. *)
-
-Reserved Notation "T |> T'" (at level 90, right associativity).
-Section TableauxExpansion.
-  Context `{set_nat : set nat} {pred func var : Atom} (sko : Skolemization_ pred func var).
-
-  Let Con := Con_ pred func var.
-  Let Form := Form_ pred func var.
-  Let Term := Term_ func var.
-
-  (** *** [ExpansionTableau] *)
-  Section Def.
-    (** We define an [ExpansionTableau] as a simple list of contexts. *)
-    (* TODO: add a [sko_record] in the definition. *)
-    Definition ExpansionTableau := list Con.
-
-    (** Make an [ExpansionTableau] from a single [Con]. *)
-    Definition mkExpansionTableau (Gamma : Con) : ExpansionTableau := [Gamma].
-
-    (** Then, a [Branch] is simply a [Con]. *)
-    Definition Branch := Con.
-
-    (** We say that [B] is the [nth_branch_of T] if [T.(i)] is [B]. *)
-    Definition nth_branch_of (T : ExpansionTableau) (i : nat) : option Branch := T.(i).
-
-    (** A branch [B] contains [F] is [F \in B]. *)
-    Definition branch_contains (B : Branch) (F : Form) : Prop := F \in B.
-
-    (** To add [F] in a branch [B] in an [ExpansionTableau] [T], it suffices to replace
-        [B] by by [F :: B]. *)
-    Definition add_in_branch
-      (T : ExpansionTableau) (i : nat) (F : Form) : ExpansionTableau :=
-      match nth_branch_of T i with
-      | None => T
-      | Some B => replace_nth i (B ,, F) T
-      end.
-
-    Definition add_branch (T : ExpansionTableau) (F : Form) (B : Branch) : ExpansionTableau :=
-      (B ,, F) :: T.
-
-    Definition branch_to_con (B : Branch) : Con := B.
-
-    Definition has_satisfiable_branch
-      (T : ExpansionTableau) (M : Model pred func) (mu : env M var) :=
-      exists (B : Branch), List.In B T /\ [[ M # [] # mu '|= ctx_to_form (branch_to_con B) ]].
-
-    (** An [ExpansionTableau] is said [satisfiable] if one of its branches is satisfiable. *)
-    Definition is_satisfiable_ExpansionTableau (T : ExpansionTableau) : Prop :=
-      exists (M : Model pred func), forall (mu : env M var), has_satisfiable_branch T M mu.
-
-    (** An [ExpansionTableau] is said [closed] if there exists a substitution [sigma] such that
-        every branch of [T] has a contradiction. *)
-    Definition is_closed_ExpansionTableau (T : ExpansionTableau) :=
-      exists (sigma : Substitution var Term),
-        List.Forall
-          (fun B => branch_contains B Bot \/
-                   exists (P P' : Form),
-                     branch_contains B P /\ branch_contains B P' /\
-                       (Neg P')@[sigma] = P@[sigma]) T.
-
-    (** If a context is satisfiable, then so is its associated [ExpansionTableau]. *)
-    Lemma ctx_satisfiable_ExpansionTableau_satisfiable :
-      forall (Gamma : Con),
-        is_satisfiable (ctx_to_form Gamma) ->
-        is_satisfiable_ExpansionTableau (mkExpansionTableau Gamma).
-    Proof using Type.
-      intros ? (M & hinterp). exists M; intro mu; exists Gamma; split.
-      - now left.
-      - apply hinterp.
-    Qed.
-
-    Lemma is_satisfiable_is_satisfiable_add_in_branch :
-      forall (T : ExpansionTableau) (B : Branch) (F G : Form) (i : nat),
-        nth_branch_of T i = Some B ->
-        is_satisfiable_ExpansionTableau T -> branch_contains B F -> imply F G ->
-        is_satisfiable_ExpansionTableau (add_in_branch T i G).
-    Proof using Type.
-      intros ????? ei (M & hsat) hcontains himp. exists M; intro mu. specialize (hsat mu).
-      destruct hsat as (B0 & hin & hinterp). apply In_nth_error in hin; destruct hin as (j & ej).
-      destruct (i == j); subst.
-      - unfold nth_branch_of in ei; rewrite ei in ej; injection ej => eB; clear ej; subst.
-        exists (B0 ,, G); split.
-        + unfold add_in_branch, nth_branch_of. rewrite ei.
-          eapply In_replace_nth; eauto.
-        + eapply extend_with_imply_form; eauto.
-      - exists B0; split; auto.
-        unfold add_in_branch; rewrite ei. eapply In_replace_nth'; eauto.
-    Qed.
-
-    Lemma is_satisfiable_is_satisfiable_or :
-      forall (T : ExpansionTableau) (B : Branch) (F G : Form) (i : nat),
-        nth_branch_of T i = Some B -> branch_contains B (Or F G) ->
-        is_satisfiable_ExpansionTableau T ->
-        is_satisfiable_ExpansionTableau (add_branch (add_in_branch T i F) G B).
-    Proof using Type.
-      intros ????? ei hcontains (M & hsat). exists M; intro mu. specialize (hsat mu).
-      destruct hsat as (B0 & hin & hinterp). apply In_nth_error in hin; destruct hin as (j & ej).
-      destruct (i == j); subst.
-      - unfold nth_branch_of in ei; rewrite ei in ej; injection ej => eB; clear ej; subst.
-        have hinterpOr := in_form_list_interp hcontains hinterp.
-        cbn in hinterpOr. destruct hinterpOr as [hF | hG].
-        + exists (B0 ,, F); split.
-          * right. unfold add_in_branch, nth_branch_of. rewrite ei.
-            eapply In_replace_nth; eauto.
-          * cbn; intros [hnF | hnB0]; auto.
-        + exists (B0 ,, G); split.
-          * now left.
-          * cbn; intros [hnG | hnB0]; auto.
-      - exists B0; split; auto. right. unfold add_in_branch. rewrite ei.
-        eapply In_replace_nth'; eauto.
-    Qed.
-
-    Lemma add_in_branch_get :
-      forall (T : ExpansionTableau) (B : Branch) (i : nat) (F : Form),
-        nth_branch_of T i = Some B ->
-        nth_branch_of (add_in_branch T i F) i = Some (B ,, F).
-    Proof using Type.
-      intros ???? e; unfold nth_branch_of in e |- *.
-      unfold add_in_branch, nth_branch_of; rewrite e.
-      erewrite get_replace_nth; eauto.
-    Qed.
-
-    Lemma add_in_branch_get' :
-      forall (T : ExpansionTableau) (B : Branch) (i j : nat) (F : Form),
-        nth_branch_of T i = Some B -> i <> j ->
-        nth_branch_of (add_in_branch T j F) i = Some B.
-    Proof using Type.
-      intros ????? e ne; unfold nth_branch_of in e |- *.
-      unfold add_in_branch, nth_branch_of.
-      destruct (T.(j)) eqn:ej; auto.
-      apply get_replace_nth'; auto.
-    Qed.
-
-    Lemma add_in_branch_get_inv' :
-      forall (T : ExpansionTableau) (B : Branch) (i j : nat) (F : Form),
-        nth_branch_of (add_in_branch T j F) i = Some B -> i <> j ->
-         nth_branch_of T i = Some B.
-    Proof using Type.
-      intros ????? e ne; unfold nth_branch_of in e |- *.
-      unfold add_in_branch, nth_branch_of in e.
-      destruct (T.(j)) eqn:ej; auto.
-      eapply get_replace_nth_inv'; eauto.
-    Qed.
-
-    Lemma add_branch_get :
-      forall (T : ExpansionTableau) (B B' : Branch) (i : nat) (F : Form),
-        nth_branch_of T i = Some B ->
-        nth_branch_of (add_branch T F B') (S i) = Some B.
-    Proof using Type.
-      intros ????? e. unfold nth_branch_of in e |- *.
-      unfold add_branch; now cbn.
-    Qed.
-
-    (* Lemma add_branch_get_inv' : *)
-    (*   forall (T : ExpansionTableau) (B B' : Branch) (i j : nat) (F : Form), *)
-    (*     nth_branch_of (add_branch T F B') i = Some B -> j <> Nat.pred i -> *)
-    (*     nth_branch_of T i = Some B. *)
-
-    Lemma branch_contains_add :
-      forall (B : Branch) (F G : Form),
-        branch_contains B F -> branch_contains (B ,, G) F.
-    Proof using Type. intros. now right. Qed.
-
-    Definition swap (i j : nat) (T : ExpansionTableau) : ExpansionTableau :=
-      match nth_branch_of T i, nth_branch_of T j with
-      | Some Bi, Some Bj =>
-          replace_nth i Bj (replace_nth j Bi T)
-      | _, _ => T
-      end.
-
-    Lemma in_tableau_in_swap :
-      forall (T : ExpansionTableau) (B : Branch) (i j : nat),
-        List.In B T <-> List.In B (swap i j T).
-    Proof using Type.
-      intros ????. split; intro hin.
-      - unfold swap, nth_branch_of.
-        destruct (T.(i)) eqn:ei, (T.(j)) eqn:ej; cbn in *; auto.
-        destruct (c0 == B).
-        + destruct (replace_nth_Some i j c c T ei).
-          subst; eapply In_replace_nth; eauto.
-        + destruct (c == B); subst.
-          * destruct (i == j); subst.
-            -- rewrite ei in ej; congruence.
-            -- rewrite replace_nth_replace_nth; auto.
-               destruct (replace_nth_Some j i c0 c0 T ej).
-               subst; eapply In_replace_nth; eauto.
-          * apply In_nth_error in hin. destruct hin as (k & ek).
-            have h0 : k <> i.
-            { intro e. rewrite -e ek in ei. congruence. }
-            have h1 : k <> j.
-            { intro e. rewrite -e ek in ej. congruence. }
-            apply In_replace_nth' with (n := k); auto.
-            apply get_replace_nth'; auto.
-      - unfold swap, nth_branch_of in hin.
-        destruct (T.(i)) eqn:ei, (T.(j)) eqn:ej; cbn in *; auto.
-        destruct (B == c0).
-        + rewrite -e in ej. eapply nth_error_In; eauto.
-        + destruct (B == c).
-          * rewrite -e in ei. eapply nth_error_In; eauto.
-          * do 2 (apply In_In_replace_nth in hin; auto).
-    Qed.
-  End Def.
-  (* We make these opaque as we provide everything needed in the API. *)
-  #[global] Opaque ExpansionTableau.
-  #[global] Opaque Branch.
-
-  (** *** Expansion Sequence *)
-
-  (** We give a relation between [ExpansionTableau] that mirrors the rules of
-      [hasTableau_] *)
-  Inductive ExpansionStep : ExpansionTableau -> ExpansionTableau -> Prop :=
-  | expansion_NegNeg :
-    forall (T : ExpansionTableau) (B : Branch) (F : Form) (i : nat),
-      nth_branch_of T i = Some B -> branch_contains B (Neg (Neg F)) ->
-      T |> (add_in_branch T i F)
-  | expansion_NegOr :
-    forall (T : ExpansionTableau) (B : Branch) (F1 F2 : Form) (i : nat),
-      nth_branch_of T i = Some B -> branch_contains B (Neg (Or F1 F2)) ->
-      T |> (add_in_branch (add_in_branch T i (Neg F1)) i (Neg F2))
-  | expansion_Or :
-    forall (T : ExpansionTableau) (B : Branch) (F1 F2 : Form) (i : nat),
-      nth_branch_of T i = Some B -> branch_contains B (Or F1 F2) ->
-      T |> (add_branch (add_in_branch T i F1) F2 B)
-  | expansion_All :
-    forall (T : ExpansionTableau) (B : Branch) (F : Form) (i : nat) (x : var),
-      nth_branch_of T i = Some B -> branch_contains B (All F) ->
-      T |> (add_in_branch T i (F {0 \to Free x}))
-  | expansion_NegAll :
-    forall (T : ExpansionTableau) (B : Branch) (F : Form) (i : nat) (t : Term)
-      (symbs : sko_record sko),
-      sko t (Neg (All F)) symbs (branch_to_con B) = true ->
-      nth_branch_of T i = Some B -> branch_contains B (Neg (All F)) ->
-      T |> (add_in_branch T i (Neg F {0 \to t}))
-  where "T |> T'" := (ExpansionStep T T').
-
-  (** An [ExpansionSequence] is a list of [ExpansionTableau] where each element is related
-      to another w.r.t. [ExpansionStep]. *)
-  Record ExpansionSequence :=
-    { seq :> list ExpansionTableau
-    ; isSequence :
-      forall (i : nat) (T T' : ExpansionTableau),
-        nth_error seq i = Some T -> nth_error seq (S i) = Some T' -> T |> T' }.
-
-  (** Expanding an [ExpansionTableau] keeps satisfiability. *)
-  Lemma satisfiable_Expansion :
-    forall (T T' : ExpansionTableau),
-      is_satisfiable_ExpansionTableau T -> (T |> T') ->
-      is_satisfiable_ExpansionTableau T'.
-  Proof using set_nat.
-    intros T T' hsat hred. induction hred.
-
-    (* Case: [Neg (Neg F)] *)
-    - eapply is_satisfiable_is_satisfiable_add_in_branch; eauto.
-      apply equiv_imply. symmetry; apply neg_neg_equiv.
-
-    (* Case: [Neg (Or F1 F2)] *)
-    - eapply is_satisfiable_is_satisfiable_add_in_branch with
-        (F := Neg (Or F1 F2)) (T := add_in_branch T i (Neg F1)).
-      + eapply add_in_branch_get; eauto.
-      + eapply is_satisfiable_is_satisfiable_add_in_branch; eauto.
-        intros M sigma hinterp hF1. apply hinterp. now left.
-      + now apply branch_contains_add.
-      + intros M sigma hinterp hF2. apply hinterp. now right.
-
-    (* Case: [Or F1 F2] *)
-    - apply is_satisfiable_is_satisfiable_or; auto.
-
-    (* Case: [All F] *)
-    - eapply is_satisfiable_is_satisfiable_add_in_branch; eauto.
-      apply instantiate_imply_all. unfold isLocallyClosed; now cbn.
-
-    (* Case: [Neg (All F)] *)
-    - destruct hsat as (M & hsat0).
-      destruct (is_sko_sound H M) as (interp & hinterpsko & hinterp).
-      exists (ReplacementModel M interp); intro mu.
-      specialize (hsat0 mu). destruct hsat0 as (B0 & hin & hinterp0).
-      apply In_nth_error in hin; destruct hin as (k & ek).
-      destruct (i == k); subst.
-      + exists (B ,, Neg F {0 \to t}); split.
-        * unfold add_in_branch. rewrite H0.
-          eapply In_replace_nth; eauto.
-        * have eB0 : B = B0.
-          { unfold nth_branch_of in H0; rewrite H0 in ek; now injection ek. }
-          intros [hnF | hB].
-          -- apply hnF, hinterpsko.
-             eapply in_form_list_interp; eauto.
-             now rewrite eB0.
-          -- rewrite eB0 in hB; now apply hB, hinterp.
-      + exists B0; split.
-        * unfold add_in_branch. rewrite H0.
-          eapply In_replace_nth'; eauto.
-        * now apply hinterp.
-  Qed.
-
-  (** Actually, two tableaux linked via an expansion are equisatisfiable. Even more important:
-      the model of the second tableau is also a model of the first tableau. *)
-  Lemma satisfiable_rev_Expansion :
-    forall (T T' : ExpansionTableau) (M : Model pred func) (mu : env M var),
-      has_satisfiable_branch T' M mu -> (T |> T') ->
-      has_satisfiable_branch T M mu.
-  Proof using Type.
-    intros ???? (B & hin & hinterp) hred; destruct hred.
-
-    (* TODO: factorize boilerplate code *)
-
-    (* Case: [Neg [Neg F]] *)
-    - destruct (In_nth_error _ _ hin) as (k & ek).
-      destruct (i == k).
-      + rewrite e in ek, H.
-        change (nth_branch_of (add_in_branch T k F) k = Some B) in ek.
-        erewrite add_in_branch_get in ek; eauto.
-        exists B0; split.
-        * eapply nth_error_In; eauto.
-        * injection ek => ek'. rewrite -ek' in hinterp; cbn in hinterp |- *.
-          apply NNPP => save; apply hinterp; now right.
-      + exists B; split; auto.
-        eapply add_in_branch_get_inv' in ek; eauto.
-        now apply nth_error_In in ek.
-
-    (* Case: [Neg [Or F1 F2]] *)
-    - destruct (In_nth_error _ _ hin) as (k & ek).
-      destruct (i == k).
-      + rewrite e in ek, H.
-        change (nth_branch_of (add_in_branch (add_in_branch T k (Neg F1)) k (Neg F2)) k = Some B)
-          in ek.
-        unshelve erewrite add_in_branch_get in ek.
-        * exact (B0 ,, Neg F1).
-        * exists B0; split.
-          -- eapply nth_error_In; eauto.
-          -- injection ek => ek'. rewrite -ek' in hinterp; cbn in hinterp |- *.
-             apply NNPP => save; apply hinterp. right; intro h; apply h; now right.
-        * now apply add_in_branch_get.
-      + exists B; split; auto.
-        do 2 eapply add_in_branch_get_inv' in ek; eauto.
-        now apply nth_error_In in ek.
-
-    (* Case: [Or F1 F2] *)
-    - destruct (In_nth_error _ _ hin) as (k & ek).
-      destruct (i == Nat.pred k).
-      + destruct k.
-        * cbn in ek. exists B0; split.
-          -- eapply nth_error_In; eauto.
-          -- injection ek => ek'; rewrite -ek' in hinterp; cbn in hinterp |- *.
-             apply NNPP => save; apply hinterp; now right.
-        * cbn in e; subst.
-          change (nth_branch_of (add_branch (add_in_branch T k F1) F2 B0) (S k) = Some B)
-            in ek.
-          unshelve erewrite add_branch_get in ek.
-          -- exact (B0 ,, F1).
-          -- exists B0; split.
-             ++ eapply nth_error_In; eauto.
-             ++ injection ek => ek'; rewrite -ek' in hinterp; cbn in hinterp |- *.
-                apply NNPP => save; apply hinterp; now right.
-          -- erewrite add_in_branch_get; eauto.
-      + destruct k.
-        * exists B0; split.
-          ++ eapply nth_error_In; eauto.
-          ++ injection ek => ek'; rewrite -ek' in hinterp; cbn in hinterp |- *.
-             apply NNPP => save; apply hinterp; now right.
-        * cbn in n, ek. exists B; split; auto.
-          eapply add_in_branch_get_inv' in ek; eauto.
-          now apply nth_error_In in ek.
-
-    (* Case: [All F] *)
-    - destruct (In_nth_error _ _ hin) as (k & ek).
-      destruct (i == k).
-      + rewrite e in ek, H.
-        change (nth_branch_of (add_in_branch T k (F {0 \to Free x})) k = Some B) in ek.
-        erewrite add_in_branch_get in ek; eauto.
-        exists B0; split.
-        * eapply nth_error_In; eauto.
-        * injection ek => ek'. rewrite -ek' in hinterp; cbn in hinterp |- *.
-          apply NNPP => save; apply hinterp; now right.
-      + exists B; split; auto.
-        eapply add_in_branch_get_inv' in ek; eauto.
-        now apply nth_error_In in ek.
-
-    (* Case: [Neg (All F)] *)
-    - destruct (In_nth_error _ _ hin) as (k & ek).
-      destruct (i == k).
-      + rewrite e in ek, H.
-        change (nth_branch_of (add_in_branch T k (Neg F {0 \to t})) k = Some B) in ek.
-        rewrite (add_in_branch_get _ B0) in ek; auto.
-        * now rewrite -e.
-        * exists B0; split.
-          --  eapply nth_error_In; eauto.
-          -- injection ek => ek'. rewrite -ek' in hinterp; cbn in hinterp |- *.
-             apply NNPP => save; apply hinterp; now right.
-      + exists B; split; auto.
-        eapply add_in_branch_get_inv' in ek; eauto.
-        now apply nth_error_In in ek.
-  Qed.
-
-  Lemma isSequence_nil :
-    forall (i : nat) (T T' : ExpansionTableau),
-      [].(i) = Some T ->
-      [].(S i) = Some T' -> T |> T'.
-  Proof using Type. intros ??? contra. rewrite nth_error_nil in contra; inversion contra. Qed.
-
-  Lemma isSequence_tail :
-    forall (s : ExpansionSequence) (T0 : ExpansionTableau) (s' : list ExpansionTableau)
-      (i : nat) (T T' : ExpansionTableau),
-      seq s = T0 :: s' -> s'.(i) = Some T -> s'.(S i) = Some T' -> T |> T'.
-  Proof using Type.
-    intros ?????? es eT eT'. apply (isSequence s (S i)); rewrite !es; cbn; auto.
-  Qed.
-
-  Lemma isSequence_singleton :
-    forall (T0 : ExpansionTableau) (i : nat) (T T' : ExpansionTableau) (Gamma : Con),
-      [T0].(i) = Some T ->
-      [T0].(S i) = Some T' -> T |> T'.
-  Proof using Type.
-    intros ?????? contra. cbn in contra; rewrite nth_error_nil in contra.
-    inversion contra.
-  Qed.
-
-  Lemma isSequence_cons :
-    forall (i : nat) (T0 T T' : ExpansionTableau) (Gamma : Con) (seq : ExpansionSequence),
-      hd_error seq = Some T0 ->
-      (mkExpansionTableau Gamma |> T0) ->
-      (mkExpansionTableau Gamma :: seq).(i) = Some T ->
-      (mkExpansionTableau Gamma :: seq).(S i) = Some T' -> T |> T'.
-  Proof using Type.
-    intros ?????? e hexpand eT eT'.
-    destruct i as [|j].
-    - cbn in eT. rewrite nth_error_cons_succ nth_error_0 in eT'.
-      rewrite e in eT'; injection eT => <-; injection eT' => <- //.
-    - have h := isSequence seq0; eapply h; eauto.
-  Qed.
-
-  Lemma expand_NegNeg :
-    forall (Gamma : Con) (F : Form),
-      Neg (Neg F) \in Gamma ->
-      mkExpansionTableau Gamma |> mkExpansionTableau (Gamma,, F).
-  Proof using Type.
-    intros ?? hin. apply (expansion_NegNeg (mkExpansionTableau Gamma) Gamma F 0); auto.
-  Qed.
-
-  Lemma expand_NegOr :
-    forall (Gamma : Con) (F1 F2 : Form),
-      Neg (Or F1 F2) \in Gamma ->
-      mkExpansionTableau Gamma |> mkExpansionTableau ((Gamma,, Neg F1),, Neg F2).
-  Proof using Type.
-    intros ??? hin. apply (expansion_NegOr (mkExpansionTableau Gamma) Gamma F1 F2 0); auto.
-  Qed.
-
-  Lemma expand_All :
-    forall (Gamma : Con) (F : Form) (x : var),
-      All F \in Gamma ->
-      mkExpansionTableau Gamma |> mkExpansionTableau (Gamma ,, F{0 \to Free x}).
-  Proof using Type.
-    intros ??? hin. apply (expansion_All (mkExpansionTableau Gamma) Gamma F 0 x); auto.
-  Qed.
-
-  Lemma expand_NegAll :
-    forall (Gamma : Con) (F : Form) (t : Term) (symbs : sko_record sko),
-      sko t (Neg (All F)) symbs Gamma = true -> Neg (All F) \in Gamma ->
-      mkExpansionTableau Gamma |> mkExpansionTableau (Gamma ,, Neg F{0 \to t}).
-  Proof using Type.
-    intros ???? hsko hin. apply (expansion_NegAll (mkExpansionTableau Gamma) Gamma F 0 t symbs hsko);
-      auto.
-  Qed.
-
-  (** Every [ExpansionTableau] of a sequence is satisfiable as long as its first tableau is
-      satisfiable. *)
-  Lemma satisfiable_ExpansionSequence :
-    forall (seq : ExpansionSequence) (T : ExpansionTableau),
-      hd_error seq = Some T -> is_satisfiable_ExpansionTableau T ->
-      forall (i : nat) (T' : ExpansionTableau),
+  (** By induction, it directly implies that if the first tableau of an expansion sequence
+      is satisfied, then all the successive tableaux are satisfied. *)
+  Lemma satisfiable_tableau_satisfiable_expansion_sequence :
+    forall (seq : Sequence sko) (T : Tableau),
+      is_expansion_sequence seq -> hd_error seq = Some T -> is_tableau_satisfiable T ->
+      forall (i : nat) (T' : Tableau),
         seq.(i) = Some T' ->
-        is_satisfiable_ExpansionTableau T'.
+        is_tableau_satisfiable T'.
   Proof using set_nat.
-    intros seq T e hsat i. induction i as [|i' IHi']; intros T' e'.
+    intros seq T hisseq e hsat i. induction i as [|i' IHi']; intros T' e'.
     - rewrite nth_error_0 e in e'. injection e' => <- //.
-    - have [T0 eT0] : exists (T0 : ExpansionTableau), seq.(i') = Some T0.
+    - have [T0 eT0] : exists (T0 : Tableau), seq.(i') = Some T0.
       { have hlt := nth_error_Some' _ _ _ e'.
         exists (nth i' seq T). apply nth_error_nth'. lia. }
-      specialize (IHi' T0 eT0). eapply satisfiable_Expansion; eauto.
-      apply (isSequence seq i' T0 T'); auto.
+      specialize (IHi' T0 eT0). eapply satisfiable_expansion_satisfiable; eauto.
   Qed.
 
-  (** In fact, there exists a model that satisfies every tableau of an [ExpansionSequence]:
-      the model of the last [ExpansionTableau] of the sequence. *)
-  Lemma model_ExpansionSequence :
-    forall (seq : ExpansionSequence) (T : ExpansionTableau),
-      hd_error seq = Some T -> is_satisfiable_ExpansionTableau T ->
-      exists (M : Model pred func), forall (mu : env M var) (i : nat) (T' : ExpansionTableau),
-        seq.(i) = Some T' ->
-        has_satisfiable_branch T' M mu.
-  Proof using set_nat.
-    intros seq ? eseq hsat.
-    have hsat' := satisfiable_ExpansionSequence seq T eseq hsat (#|seq| - 1).
-    have [T' eT'] : exists T', seq.(#|seq| - 1) = Some T'.
-    { have esome := nth_error_Some seq (#|seq| - 1).
-      have hlt : #|seq| - 1 < #|seq|.
-      { rewrite PeanoNat.Nat.sub_1_r. destruct seq, seq0.
-        - cbn in eseq. inversion eseq.
-        - cbn. lia. }
-      rewrite -esome in hlt.
-      destruct (seq.(#|seq| - 1)).
-      - exists e; auto.
-      - exfalso; now apply hlt. }
-    specialize (hsat' T' eT'). destruct hsat' as (M & hsat'). exists M; intro mu; specialize (hsat' mu).
-    clear hsat.
-
-    enough (h : forall (i : nat) (T0 : ExpansionTableau),
-               seq.(#|seq| - (S i)) = Some T0 -> has_satisfiable_branch T0 M mu).
-    { intros ? T0 e. specialize (h (#|seq| - 1 - i)).
-      have e0 : #| seq | - S (#| seq | - 1 - i) = i.
-      { rewrite PeanoNat.Nat.sub_1_r Arith_base.minus_Sn_m_stt.
-        - apply nth_error_Some' in e; lia.
-        - rewrite PeanoNat.Nat.sub_sub_distr.
-          + apply nth_error_Some' in e; lia.
-          + have hseq : #|seq| > 0.
-            { apply nth_error_Some' in e; destruct i; lia. }
-            lia.
-          + rewrite PeanoNat.Nat.succ_pred.
-            * intro; apply nth_error_Some' in e; lia.
-            * rewrite PeanoNat.Nat.sub_diag //. }
-      rewrite e0 in h; eapply h; eauto. }
-
-    intro i; induction i as [|i' IHi'].
-    - now intros T0 e0; rewrite e0 in eT'; injection eT' => ->.
-    - intros T0 eT0.
-      have [T0' eT0'] : exists T0', seq.(#|seq| - S i') = Some T0'.
-      { have h0 : #|seq| > 0 by apply nth_error_Some' in eT'; lia.
-        have h : #|seq| - S i' < #|seq| by lia.
-        destruct (seq.(#|seq| - S i')) eqn:T0'.
-        - exists e; auto.
-        - rewrite nth_error_None in T0'; lia. }
-      specialize (IHi' T0' eT0').
-      destruct (Compare_dec.dec_le (S (S i')) #|seq|).
-      + have hred : T0 |> T0'.
-        { apply (isSequence seq) with (i := #|seq| - S (S i')); auto.
-          rewrite Arith_base.minus_Sn_m_stt //. }
-        eapply satisfiable_rev_Expansion; eauto.
-      + apply Compare_dec.not_le in H. unfold gt, lt in H.
-        have hle' := le_S_n _ _ H.
-        have hle : #|seq| <= S (S i') by apply le_S.
-        rewrite -!PeanoNat.Nat.sub_0_le in hle, hle'.
-        rewrite hle in eT0; rewrite hle' in eT0'.
-        rewrite eT0 in eT0'; injection eT0' => -> //.
-  Qed.
-
-  Lemma satisfiable_ExpansionSequence_hasTableau_satisfiable :
-    forall (Gamma : Con) (sigma : Substitution var Term) (T : hasTableau sko Gamma sigma),
-      is_satisfiable (ctx_to_form Gamma) ->
-      exists (M : Model pred func), forall (mu : env M var),
-        is_tableau_satisfiable M mu T.
-  Proof.
-    intros ??? hsat.
-
-    have hsat0 : is_satisfiable_ExpansionTableau (mkExpansionTableau Gamma).
-    { destruct hsat as (M & hsat); exists M; intro mu. specialize (hsat mu).
-      exists Gamma; split; auto. now left. }
-
-    set seq := hasTableau_has_ExpansionSequence T.
-
-    have [M hseq] := model_ExpansionSequence (proj1_sig seq) (mkExpansionTableau Gamma)
-                       (proj2_sig seq) hsat0.
-    exists M; intro mu. specialize (hseq mu).
-
-    (* This is the nice hypothesis for [Or]. *)
-    have hinterpGamma : interpret_form_ M [] mu (ctx_to_form Gamma).
-    { destruct (hseq 0 (mkExpansionTableau Gamma) (proj2_sig seq)) as (B & hin & hinterp);
-        destruct hin as [e | contra]; [|inversion contra].
-      rewrite e //. }
-    change [[ M # [] # mu '|= ctx_to_form Gamma ]] in hinterpGamma.
-
-    (* TODO: find the nice hypothesis for [Neg (All F)]. *)
-
-    (* have hinterpCanonical : *)
-    (*   forall (F : Form) (t : Term) (symbs : sko_record sko), *)
-    (*     (proj1_sig seq).(1) = Some (mkExpansionTableau (Gamma ,, Neg F{0 \to t})) -> *)
-    (*     sko t (Neg (All F)) symbs Gamma = true -> Neg (All F) \in Gamma -> *)
-    (*     interpret_form_ M [] mu (Neg F{0 \to t}). *)
-    (* { intros; induction T; try inversion H. *)
-    (*   - have e := proj2_sig (hasTableau_has_ExpansionSequence T). *)
-    (*     unfold hd_error in e. rewrite e in H3; injection H3 => contra. *)
-
-    clear hsat hsat0; induction T.
-
-    (* Case: [Bot] *)
-    - have [] := in_form_list_interp i hinterpGamma.
-
-    (* Case: contradiction *)
-    - now constructor.
-
-    (* Case: [Neg (Neg F)]. *)
-    - constructor; apply IHT.
-      + intros k T'. rewrite -hasTableau_has_ExpansionSequence_NegNeg -nth_error_S; intro.
-        eapply hseq; eauto.
-      + eapply extend_with_equiv_form; eauto; apply neg_neg_equiv.
-
-    (* Case: [Neg (Or F1 F2)] *)
-    - constructor; apply IHT.
-      + intros k T'. rewrite -hasTableau_has_ExpansionSequence_NegOr -nth_error_S; intro.
-        eapply hseq; eauto.
-      + apply interp_list_commute; eapply extend_with_equiv_form; eauto.
-        apply neg_equiv; etransitivity; [apply or_comm|]; apply or_equiv; symmetry;
-          apply neg_neg_equiv.
-
-    (* Case: [Or F1 F2] *)
-    - have hor := in_form_list_interp i hinterpGamma; cbn in hor; destruct hor as [hF1 | hF2].
-      + constructor; apply IHT1.
-        * admit.
-        * cbn; now intros [].
-      + constructor; apply IHT2.
-        * admit.
-        * cbn; now intros [].
-
-    (* Case: [All F] *)
-    - constructor; apply IHT. eapply extend_with_imply_form; eauto; apply instantiate_imply_all.
-      now cbn.
-
-    (* Case: [Neg (All F)] *)
-    - constructor; apply IHT.
-    Admitted.
-End TableauxExpansion.
-
-Section TableauxSoundness.
-  Context `{set_nat : set nat} {pred func var : Atom} (sko : Skolemization_ pred func var).
-
-  Let Con := Con_ pred func var.
-  Let Form := Form_ pred func var.
-  Let Term := Term_ func var.
-
-  (** We start by showing that if the root formula of a tableau is satisfiable, then this
-      tableau is also satisfiable.
-
-      Note that [Gamma] must be a closed context. *)
-  Lemma hasTableau_satisfiable :
-    forall {Gamma : Con} {sigma : Substitution var Term} (T : hasTableau sko Gamma sigma)
-      (M : Model pred func),
-      (forall  (mu : env M var), [[ M # [] # mu '|= ctx_to_form Gamma ]]) ->
-      exists (M' : Model pred func), forall (mu' : env M' var),
-        is_tableau_satisfiable M' mu' T.
-  Proof using Type.
-    intros ???? hinterp.
-
-    have htab : exists (sigma : Substitution var Term), hasTableau sko Gamma sigma by exists sigma.
-    apply hasTableau_has_ExpansionSequence in htab.
-    destruct htab as (seq & e & _).
-    have h0 : is_satisfiable (ctx_to_form Gamma) by now exists M.
-    eapply satisfiable_ExpansionSequence_hasTableau_satisfiable; eauto.
-  Qed.
-
-  (** Of course, no tableau is satisfiable. We start by showing 2 small lemmas: *)
-  Lemma in_ctx_in_substituted_ctx :
-    forall (Gamma : Con) (F : Form) (sigma : Substitution var Term),
-      F \in Gamma -> F@[sigma] \in Gamma@[sigma].
-  Proof using Type.
-    intros ???. induction Gamma as [|G Gs IHGs]; intros Hin; inversion Hin.
-    - rewrite H. cbn. now left.
-    - right. now apply IHGs.
-  Qed.
-
-  Lemma subst_ctx_subst_list :
-    forall (Gamma : Con) (sigma : Substitution var Term),
-      (ls_to_form Gamma)@[sigma] = ls_to_form (Gamma@[sigma]).
-  Proof using Type.
-    intros; cbn. induction Gamma as [|F Fs IHFs]; auto.
-    cbn. do 3 f_equal. apply IHFs.
-  Qed.
-
-  Lemma hasTableau_not_satisfiable :
-    forall (M : Model pred func)
-      {Gamma : Con} {symbs : sko_record sko} {sigma : Substitution var Term}
-      (T : hasTableau_ sko Gamma symbs sigma), is_tableau_satisfiable M (subst_to_env M sigma) T -> False.
-  Proof using Type.
-    intros ????? hsat. remember (subst_to_env M sigma) as mu. induction hsat.
-    2-7: now apply IHhsat.
-    subst. rewrite -subst_commutes_with_env_forms in H.
-    have h1 : interpret_form_ M [] (empty_env M var) P@[sigma].
-    { eapply in_form_list_interp.
-      - apply in_ctx_in_substituted_ctx; eauto.
-      - rewrite -subst_ctx_subst_list //. }
-    have h2 : interpret_form_ M [] (empty_env M var) (Neg P)@[sigma].
-    { eapply in_form_list_interp.
-      - cbn; rewrite e. apply in_ctx_in_substituted_ctx; eauto.
-      - rewrite -subst_ctx_subst_list //. }
-    cbn in h2. now apply h2.
-  Qed.
-
+  (** This allows us to deduce the the soundness theorem. *)
   Theorem hasTableau_sound :
-    forall (sigma : Substitution var Term) (Gamma : Con) (F : Form),
-      isClosed (Gamma ,, Neg F) ->
-      hasTableau sko (Gamma ,, Neg F) sigma -> Gamma |= F.
+    forall (sigma : Substitution var Term) (Gamma : list Form) (F : Form),
+      isClosed (Neg F :: Gamma) ->
+      hasTableau sko (Neg F :: Gamma) sigma -> Gamma |= F.
   Proof using Type.
-    intros ??? hclosedGamma htab.
+    intros ??? hclosedGamma (sequence & hproof).
     rewrite models_iff. intros M. left. intro hsat.
     have hsat' : forall (mu : env M var),
         interpret_form_ M [] mu (ls_to_form (Neg F :: Gamma)).
     { intro mu; change [[ M # [] # mu '|= ls_to_form (Neg F :: Gamma) ]].
       rewrite (isClosed_interp_form_env_eq _ _ _ _ (empty_env M var)); auto.
       rewrite isClosedList_isClosedFormList //. }
-    eapply hasTableau_satisfiable with (T := htab) in hsat'.
-    destruct hsat' as (M' & hsat'). specialize (hsat' (subst_to_env M' sigma)).
-    eapply hasTableau_not_satisfiable; eauto.
+    have hnsat := hasTableau_not_satisfiable _ _ _ _ hproof.
+    have htab : is_tableau_satisfiable (mkTableau sko (Neg F :: Gamma)).
+    { exists M. intro mu. exists []. split.
+      - apply is_branch_of_nil.
+      - apply hsat'. }
+    destruct hproof as (hisseq & e & hclosed).
+    have htabsat := satisfiable_tableau_satisfiable_expansion_sequence
+                      sequence (mkTableau sko (Neg F :: Gamma)) hisseq e htab.
+    specialize (htabsat (#|sequence| - 1)).
+    have [T' eT'] : exists (T' : Tableau), sequence.(#|sequence| - 1) = Some T'.
+    { destruct (sequence.(#|sequence| - 1)) eqn:elast.
+      - exists t; auto.
+      - exfalso. rewrite nth_error_None in elast.
+        have hlt : 0 < #|sequence|.
+        { eapply nth_error_Some'. rewrite nth_error_0. exact e. }
+        lia. }
+    specialize (htabsat T' eT'). destruct htabsat as (M' & htabsat').
+    specialize (htabsat' (subst_to_env M' sigma)). destruct htabsat' as (B & hisbranch & hsatB).
+    specialize (hnsat M' B).
+    have elast : last sequence (mkLeaf sko) = T'.
+    { destruct sequence.
+      - inversion e.
+      - clear hisseq e hclosed hisbranch hnsat. generalize dependent t.
+        induction sequence as [|T0 seq IHseq]; intros T eT.
+        + cbn in eT |- *. injection eT => -> //.
+        + apply IHseq; cbn in eT |- *. rewrite PeanoNat.Nat.sub_0_r //. }
+    rewrite -elast in hisbranch. specialize (hnsat hisbranch).
+    apply hnsat. rewrite elast //.
   Qed.
-End TableauxSoundness.
-
-Module ConcreteProofInstances.
-  Export ConcreteSkolemizationInstances.
-
-  Definition Con := Con_ string string string.
-End ConcreteProofInstances.
+End Soundness.
